

Chapter 4 Solutions

1. Consider the method of moments estimator of Example 4.6

- (a) The following data were observed: $x_1 = 1, x_2 = 1, x_3 = 7$ from the $U(0, \theta)$ distribution. Compute the method of moments estimator for θ .

Given the data $x_1 = 1, x_2 = 1, x_3 = 7$ we find $\bar{x} = 3$ and so $\hat{\theta} = 2\bar{x} = 6$.

- (b) Identify potential drawbacks of this estimator.

This estimator can sometimes be nonsense. For example, using the data from the previous part, $\hat{\theta} = 6$. However we know that θ must be bigger than all x_i 's so $\theta > 7$ which contradicts $\hat{\theta} < 7$.

2. Verify the formula from the mgf of the gamma distribution in Example 4.7 and use it to derive its mean and variance.

For the $\text{Gamma}(\alpha, \beta)$ distribution,

$$f(x|\alpha, \beta) = \frac{\beta^\alpha}{\Gamma(\alpha)} x^{\alpha-1} e^{-\beta x}.$$

Then

$$\begin{aligned} M_X(t) &= \int_0^\infty e^{tx} \frac{\beta^\alpha}{\Gamma(\alpha)} x^{\alpha-1} e^{-\beta x} dx \\ &= \int_0^\infty \frac{\beta^\alpha}{\Gamma(\alpha)} x^{\alpha-1} e^{-(\beta-t)x} dx \\ &= \frac{\beta^\alpha}{(\beta-t)^\alpha} \int_0^\infty \frac{(\beta-t)^\alpha}{\Gamma(\alpha)} x^{\alpha-1} e^{-(\beta-t)x} dx \\ &= \frac{\beta^\alpha}{(\beta-t)^\alpha}, \text{ for } t < \beta. \\ &= (1 - t/\beta)^{-\alpha}, \text{ for } t < \beta. \\ \Rightarrow M_X^{(1)}(t) &= \frac{d}{dt} M_X(t) = \frac{\alpha}{\beta} (1 - t/\beta)^{-\alpha-1} \\ \Rightarrow \mu_1 &= M_X^{(1)}(0) = \frac{\alpha}{\beta} \\ \Rightarrow M_X^{(2)}(t) &= \frac{d^2}{dt^2} M_X(t) = \frac{\alpha(\alpha+1)}{\beta^2} (1 - t/\beta)^{-\alpha-2} \end{aligned}$$

$$\Rightarrow \mu_2 = M_X^{(2)}(0) = \frac{\alpha(\alpha+1)}{\beta^2}$$

$$\Rightarrow \text{Var}(X) = \mu_2 - \mu_1^2 = \frac{\alpha(\alpha+1)}{\beta^2} - \frac{\alpha^2}{\beta^2} = \frac{\alpha}{\beta^2}.$$

3. Explain why the MLE of Example 4.10 is biased but do not derive its bias. *Hint.* Think why $\max\{X_i\} < \theta$, and what this means about $E[\max\{X_i\}]$.

Because each $X_i < \theta$, then $X_{(n)} = \max\{X_1, \dots, X_n\} < \theta$, so $E X_{(n)} < \theta$. Therefore $\text{Bias}_\theta(X_{(n)}) = E X_{(n)} - \theta < 0$. So $\text{Bias}_\theta(X_{(n)}) \neq 0$ which means that $X_{(n)}$ is biased for θ .

4. Let $X_1, \dots, X_n \stackrel{\text{iid}}{\sim} \text{Bernoulli}(\theta)$, $\theta \in (0, 1)$.

- (a) Derive the MLE for θ .

The pmf for X is

$$f(x|\theta) = \theta^x(1-\theta)^{1-x}, \quad x \in \{0, 1\}, \quad \theta \in [0, 1].$$

Taking logarithms,

$$\begin{aligned} \log f(x|\theta) &= x \log \theta + (1-x) \log(1-\theta) \\ \Rightarrow \ell(\theta|\mathbf{x}) &= \sum_{i=1}^n \log f(x_i|\theta) \\ &= \sum_{i=1}^n \{x_i \log \theta + (1-x_i) \log(1-\theta)\} \\ &= \log \theta \sum_{i=1}^n x_i + \log(1-\theta)(n - \sum_{i=1}^n x_i) \\ \Rightarrow \ell'(\theta|\mathbf{x}) &= \frac{1}{\theta} \sum_{i=1}^n x_i - \frac{1}{1-\theta} (n - \sum_{i=1}^n x_i) \\ 0 &= \frac{1}{\hat{\theta}} \sum_{i=1}^n x_i - \frac{1}{1-\hat{\theta}} (n - \sum_{i=1}^n x_i) \\ 0 &= \frac{n}{\hat{\theta}} \bar{x} - \frac{n}{1-\hat{\theta}} (1-\bar{x}) \\ 0 &= \frac{\bar{x}}{\hat{\theta}} - \frac{1-\bar{x}}{1-\hat{\theta}} \end{aligned}$$

$$\hat{\theta} = \bar{x}$$

Evaluating the second derivative of $\ell(\theta|\mathbf{x})$ at $\theta = \bar{x}$ is negative which confirms this is a maximum.